add smt

Demo/Demo.lean
@@ -3,64 +3,23 @@ import Mathlib.Tactic.Ring
 import Std
 import Demo.Util
 
-def fib : Nat → Nat
-  | 0 => 0
-  | 1 => 1
-  | n + 2 => fib (n + 1) + fib n
-
-#eval fib 5
-#eval List.range 20 |>.map fib
+def fib : Nat → Nat := sorry
 
 -- set_option trace.Meta.Tactic.simp.rewrite true in
-theorem fib_add_two {n : ℕ} : fib (n + 2) = fib n + fib (n + 1) := by
-  simp [fib, add_comm]
+-- theorem fib_add_two {n : ℕ} : fib (n + 2) = fib n + fib (n + 1) := by
+--   simp [fib, add_comm]
 
 lemma fib_add (m n : ℕ) :
-  fib (m + n + 1) = fib m * fib n + fib (m + 1) * fib (n + 1) := by
-  induction n generalizing m
-  · case zero =>
-    simp [fib]
-  · case succ n ih =>
-    intros
-    specialize ih (m + 1)
-    rw [add_assoc m 1 n, add_comm 1 n] at ih
-    simp only [fib_add_two, ih]
-    ring
+    fib (m + n + 1) = fib m * fib n + fib (m + 1) * fib (n + 1) := by
+  sorry
 
-def fib₀ : Nat → Nat
-  | 0 => 0
-  | n + 1 => (aux n).2
-where
-  aux : Nat → Nat × Nat
-    | 0 => (0, 1)
-    | n + 1 =>
-      let (a, b) := aux n
-      (b, a + b)
+def fib₀ : Nat → Nat := sorry
 
-#eval List.range 20 |>.map fib₀
-
-lemma fib₀_aux_eq (n : Nat) : fib₀.aux n = (fib n, fib (n + 1)) := by
-  induction n
-  . case zero =>
-    simp [fib]
-  . case succ n ih =>
-    simp [fib₀.aux, fib, ih, add_comm]
-
-lemma fib₀_aux_eq_alt (n : Nat) : fib₀.aux n = (fib n, fib (n + 1)) := by
-  induction n <;> simp [*, fib, fib₀.aux, add_comm]
-
-@[csimp] theorem fib₀_eq : fib = fib₀ := by
-  ext n
-  cases n <;> simp [fib₀, fib₀_aux_eq]
-
--- #eval fib₀ 1000
--- #eval fib 1000
+-- lemma fib₀_aux_eq (n : Nat) : fib₀.aux n = (fib n, fib (n + 1)) := by
 
 def fib₁ (n : Nat) :=
   aux n 0 1
-where aux : Nat → Nat → Nat → Nat
-  | 0,   a, _ => a
-  | n+1, a, b => aux n b (a + b)
+where aux : Nat → Nat → Nat → Nat := sorry
 
 -- #eval fib₁ 400000
 
@@ -71,45 +30,20 @@ def fib₂ (n : Nat) : Nat := Id.run do
     p := (b, a + b)
   return p.1
 
-def fib₃ (n : Nat) : Nat := Id.run do
-  let mut a := 0
-  let mut b := 1
-  for _ in [:n] do
-    let temp := a
-    a := b
-    b := temp + a
-  return a
-
-#eval fib₃ 100000
-
 def fib₄ (n : Nat) : { m // m = fib n } :=
   let ⟨pair, property⟩ :=
   loop_with_invariant
-    (invariant := fun i p => p = (fib i, fib (i + 1)))
+    (invariant := sorry)
     (start_state := (0, 1))
-    (init := by simp)
+    (init := sorry)
     (next_state := fun i p =>
-      let (a, b) := p
-      (b, a + b))
-    (step := by intro i; simp [fib, add_comm])
+      sorry)
+    (step := sorry)
     n
-  ⟨pair.1, by simp [property]⟩
+  sorry
 
-#eval fib₃ 100
-#eval fib₄ 100
+def fib₅ (n : Nat) : { m // m = fib n } := sorry
 
-def fib₅ (n : Nat) : { m // m = fib n } :=
-  for i upto n
-    state: p := (0, 1)
-    invariant: inv := p = (fib i, fib (i + 1))
-    init:= by simp
-    next:
-      let (a, b) := p
-      (b, a + b)
-    step:= by intro i; simp [fib, add_comm]
-  ⟨p.1, by simp [inv]⟩
-
--- #eval fib₅ 400000
 
 /-
 Notes.
