Demo/SmtDemo.lean
@@ -1,0 +1,81 @@
+import Mathlib.Data.Nat.GCD.Basic
+import Mathlib.Tactic.Ring
+import Std
+import Demo.Util
+import Smt
+import Aesop
+
+-- set_option smt.solver.path "..."
+-- set_option smt.solver.kind "vampire"
+
+example (n m : Int) (h : 0 < m) : n % m < m := by
+  smt [h]
+  sorry
+
+example (n m k l : Int) : (n - m) * k + l = n*k - m*k + l := by
+  smt
+  sorry
+
+example (n m k l : Int) (hN : n ≤ m) (hK : k ≤ l) : n + k ≤ m + l := by
+  smt [hN, hK]
+  sorry
+
+theorem cong (x y : Int) (f : Int → Int) : x = y → f x = f y := by
+  smt
+  simp_all
+
+@[aesop safe]
+def fib : Nat → Nat
+  | 0 => 0
+  | 1 => 1
+  | n + 2 => fib (n + 1) + fib n
+
+@[aesop safe]
+theorem fib_zero : fib 0 = 0 := rfl
+
+@[aesop safe]
+theorem fib_one : fib 1 = 1 := rfl
+
+@[aesop safe]
+theorem fib_add_two (n : ℕ) : fib (n + 2) = fib n + fib (n + 1) := by
+  simp [fib, add_comm]
+
+lemma fib_add (m n : ℕ) :
+    fib (m + n + 1) = fib m * fib n + fib (m + 1) * fib (n + 1) := by
+  induction n generalizing m
+  · case zero =>
+    simp [fib]
+  · case succ n ih =>
+    intros
+    specialize ih (m + 1)
+    rw [add_assoc m 1 n, add_comm 1 n] at ih
+    simp only [fib_add_two, ih]
+    ring
+
+-- lemma fib_add' (m n : ℕ) :
+--     fib (m + n + 1) = fib m * fib n + fib (m + 1) * fib (n + 1) := by
+--   induction n generalizing m
+--   · case zero =>
+--     smt [fib_zero, fib_one]
+--     sorry
+--   · case succ n ih =>
+--     intros
+--     specialize ih (m + 1)
+--     smt [fib_zero, fib_one, fib_add_two, ih]
+--     rw [add_assoc m 1 n, add_comm 1 n] at ih
+--     simp only [fib_add_two, ih]
+--     ring
+
+lemma fib_add'' (m n : ℕ) :
+    fib (m + n + 1) = fib m * fib n + fib (m + 1) * fib (n + 1) := by
+  induction n generalizing m
+  · case zero =>
+    aesop
+  · case succ n ih =>
+    intros
+    specialize ih (m + 1)
+    rw [add_assoc m 1 n, add_comm 1 n] at ih
+    simp only [fib_add_two, ih]
+    ring
+
+
