lakefile.lean
@@ -7,6 +7,7 @@ lean_lib Demo
 
 require mathlib from git"https://github.com/leanprover-community/mathlib4"@"master"
 require Cli from git"https://github.com/mhuisi/lean4-cli"@"nightly"
+require smt from git "https://github.com/ufmg-smite/lean-smt"@"main"
 
 @[default_target]
 lean_exe demo {
